Add the [debugFifo] module (with debugging messages by [Display])

Kami/Ex/Fifo.v
@@ -7,43 +7,44 @@ Require Import FunctionalExtensionality Eqdep Eqdep_dec.
 Set Implicit Arguments.
 
 Section Fifo.
-  Variable fifoName: string.
-  Variable sz: nat.
-  Variable dType: Kind.
+  Variables (fifoName: string)
+            (sz: nat)
+            (dType: Kind).
 
   Local Notation "^ s" := (fifoName -- s) (at level 0).
 
-  Definition enq {ty} : forall (d: ty dType), ActionT ty Void := fun d =>
-    (Read isFull <- ^"full";
-     Assert !#isFull;
-     Read eltT <- ^"elt";
-     Read enqPT <- ^"enqP";
-     Read deqPT <- ^"deqP";
-     Write ^"elt" <- #eltT@[#enqPT <- #d];
-     Write ^"empty" <- $$false;
-     LET next_enqP <- (#enqPT + $1) :: Bit sz;
-     Write ^"full" <- (#deqPT == #next_enqP);
-     Write ^"enqP" <- #next_enqP;
-     Retv)%kami_action.
+  Definition enq {ty} : forall (d: ty dType), ActionT ty Void :=
+    fun d =>
+      (Read isFull <- ^"full";
+      Assert !#isFull;
+      Read eltT <- ^"elt";
+      Read enqPT <- ^"enqP";
+      Read deqPT <- ^"deqP";
+      Write ^"elt" <- #eltT@[#enqPT <- #d];
+      Write ^"empty" <- $$false;
+      LET next_enqP <- (#enqPT + $1) :: Bit sz;
+      Write ^"full" <- (#deqPT == #next_enqP);
+      Write ^"enqP" <- #next_enqP;
+      Retv)%kami_action.
 
   Definition deq {ty} : ActionT ty dType :=
     (Read isEmpty <- ^"empty";
-     Assert !#isEmpty;
-     Read eltT <- ^"elt";
-     Read enqPT <- ^"enqP";
-     Read deqPT <- ^"deqP";
-     Write ^"full" <- $$false;
-     LET next_deqP <- (#deqPT + $1) :: Bit sz;
-     Write ^"empty" <- (#enqPT == #next_deqP);
-     Write ^"deqP" <- #next_deqP;
-     Ret #eltT@[#deqPT])%kami_action.
+    Assert !#isEmpty;
+    Read eltT <- ^"elt";
+    Read enqPT <- ^"enqP";
+    Read deqPT <- ^"deqP";
+    Write ^"full" <- $$false;
+    LET next_deqP <- (#deqPT + $1) :: Bit sz;
+    Write ^"empty" <- (#enqPT == #next_deqP);
+    Write ^"deqP" <- #next_deqP;
+    Ret #eltT@[#deqPT])%kami_action.
 
   Definition firstElt {ty} : ActionT ty dType :=
     (Read isEmpty <- ^"empty";
-     Assert !#isEmpty;
-     Read eltT : Vector dType sz <- ^"elt";
-     Read deqPT <- ^"deqP";
-     Ret #eltT@[#deqPT])%kami_action.
+    Assert !#isEmpty;
+    Read eltT : Vector dType sz <- ^"elt";
+    Read deqPT <- ^"deqP";
+    Ret #eltT@[#deqPT])%kami_action.
 
   Definition fifo := MODULE {
     Register ^"elt" : Vector dType sz <- Default
@@ -70,15 +71,70 @@ Section Fifo.
 
 End Fifo.
 
-Hint Unfold fifo simpleFifo : ModuleDefs.
-Hint Unfold enq deq firstElt : MethDefs.
+Hint Unfold fifo simpleFifo: ModuleDefs.
+Hint Unfold enq deq firstElt: MethDefs.
+
+Section DebugFifo.
+  Variables (fifoName: string)
+            (sz: nat)
+            (dType: Kind).
+
+  Local Notation "^ s" := (fifoName -- s) (at level 0).
+
+  Variables (enqMsg: string)
+            (enqDisp: forall ty, ty dType -> list (Disp ty))
+            (deqMsg: string)
+            (deqDisp: forall ty, ty dType -> list (Disp ty)).
+
+  Definition debugEnq {ty} : forall (d: ty dType), ActionT ty Void :=
+    fun d =>
+      (Display
+         enqMsg (enqDisp _ d)
+         (Read isFull <- ^"full";
+         Assert !#isFull;
+         Read eltT <- ^"elt";
+         Read enqPT <- ^"enqP";
+         Read deqPT <- ^"deqP";
+         Write ^"elt" <- #eltT@[#enqPT <- #d];
+         Write ^"empty" <- $$false;
+         LET next_enqP <- (#enqPT + $1) :: Bit sz;
+         Write ^"full" <- (#deqPT == #next_enqP);
+         Write ^"enqP" <- #next_enqP;
+         Retv)%kami_action).
+
+  Definition debugDeq {ty} : ActionT ty dType :=
+    (Read isEmpty <- ^"empty";
+    Assert !#isEmpty;
+    Read eltT <- ^"elt";
+    Read enqPT <- ^"enqP";
+    Read deqPT <- ^"deqP";
+    Write ^"full" <- $$false;
+    LET next_deqP <- (#deqPT + $1) :: Bit sz;
+    Write ^"empty" <- (#enqPT == #next_deqP);
+    Write ^"deqP" <- #next_deqP;
+    LET delt <- #eltT@[#deqPT];
+    Display deqMsg (deqDisp _ delt) (Ret #delt))%kami_action.
+
+  Definition debugFifo := MODULE {
+    Register ^"elt" : Vector dType sz <- Default
+    with Register ^"enqP" : Bit sz <- Default
+    with Register ^"deqP" : Bit sz <- Default
+    with Register ^"empty" : Bool <- true
+    with Register ^"full" : Bool <- Default
+
+    with Method ^"enq"(d : dType) : Void := (debugEnq d)
+    with Method ^"deq"() : dType := debugDeq
+  }.
+
+End DebugFifo.
+
+Hint Unfold debugFifo: ModuleDefs.
+Hint Unfold debugEnq debugDeq: MethDefs.
 
 Section Facts.
-  Variable fifoName: string.
-  Variable sz: nat.
-  Variable dType: Kind.
-
-  Hypothesis HfifoName: index 0 indexSymbol fifoName = None.
+  Variables (fifoName: string)
+            (sz: nat)
+            (dType: Kind).
 
   Lemma fifo_ModEquiv:
     ModPhoasWf (fifo fifoName sz dType).
@@ -99,6 +155,21 @@ Section Facts.
     ModRegsWf (simpleFifo fifoName sz dType).
   Proof. kvr. Qed.
   Hint Resolve simpleFifo_ValidRegs.
+
+  Variables (enqMsg: string)
+            (enqDisp: forall ty, ty dType -> list (Disp ty))
+            (deqMsg: string)
+            (deqDisp: forall ty, ty dType -> list (Disp ty)).
+
+  Lemma debugFifo_ModEquiv:
+    ModPhoasWf (debugFifo fifoName sz enqMsg enqDisp deqMsg deqDisp).
+  Proof. kequiv. Qed.
+  Hint Resolve debugFifo_ModEquiv.
+
+  Lemma debugFifo_ValidRegs:
+    ModRegsWf (debugFifo fifoName sz enqMsg enqDisp deqMsg deqDisp).
+  Proof. kvr. Qed.
+  Hint Resolve debugFifo_ValidRegs.
 
 End Facts.
 
